ALmost finished inversion lemma for lambda abstraction

src/main.lean
@@ -43,7 +43,13 @@ notation n"¬ε"Γ => inCtx n Γ → false
 
 inductive validCtx : Ctx → Type 
 | nil : validCtx []
-| cons (n : Nat) (A : Typ) (Γ : Ctx) : (n ¬ε Γ) → validCtx Γ → validCtx (n:A , Γ)
+| cons (n : Nat) (A : Typ) (Γ : Ctx) : (n ¬ε Γ) → validCtx Γ → validCtx (n:A , Γ) 
+
+inductive ctxSubset : Ctx → Ctx → Type 
+| nil : ctxSubset [] Γ 
+| cons : (n ε Γ') → ctxSubset Γ Γ' → ctxSubset (n:A , Γ) Γ' 
+
+notation Γ" ∼ "Γ' => (ctxSubset Γ Γ') × (ctxSubset Γ' Γ)
 
 inductive Term : Type
 | var : Nat → Term                  -- variable
@@ -108,6 +114,8 @@ inductive Deduction : Ctx → Term → Typ → Type
 notation Γ " ⊢ " t " ∶ " A => Deduction Γ t A 
 namespace Deduction
 
+theorem eqCtxEqDeduction {Γ Γ' : Ctx} : (Γ ∼ Γ') → (Γ ⊢ t ∶ A) → (Γ' ⊢ t ∶ A) := by 
+  sorry
 -- If a weakest context is valid, then a strongest one remains valid --
 theorem weakValidCtx (Γ : Ctx) (n₁ : Nat) (A₁ : Typ) : validCtx (n₁:A₁ , Γ) → validCtx Γ  := by 
   intro d 
@@ -236,7 +244,65 @@ inductive Reduction : Term → Term → Type
 
 notation t₁ "~>₁" t₂ => Reduction t₁ t₂ 
 
-theorem invAbs : (Γ ⊢ λ(n).t ∶ A->B) → ((n:A, Γ) ⊢ t ∶ B) := by sorry
+
+theorem th1 : (n:A,n₁:A₂,n₂:A₃,Γ₁) ∼ (n:A,n₂:A₃,n₁:A₂,Γ₁) := by 
+      constructor 
+      . apply ctxSubset.cons 
+        . apply inCtx.init
+        . apply ctxSubset.cons 
+          . apply inCtx.cons 
+            apply inCtx.cons 
+            apply inCtx.init 
+          . apply ctxSubset.cons 
+            . apply inCtx.cons 
+              apply inCtx.init
+            . induction Γ₁
+              case fst.a.a.a.nil => apply ctxSubset.nil 
+              case fst.a.a.a.cons n₅ A₅ Γ₅ ih => 
+                apply ctxSubset.cons 
+                . apply inCtx.cons
+                  apply inCtx.cons
+                  apply inCtx.cons
+                  apply inCtx.init
+                . sorry
+            . sorry
+-- There must be a better way to handle this without going full blown lists --
+
+
+
+
+theorem invAbs2 (Γ : Ctx) (t q : Term) (n : Nat) (A B C :Typ) : (t = λ(n).q) → (C = A->B) → (Γ ⊢ t ∶ C) → ((n:A, Γ) ⊢ q ∶ B) := by
+  intro d₁ d₂ d₃  
+  induction  d₃ 
+  case var n D => contradiction 
+  case weak t₁ A₁ n₁ Γ₁ A₂ h₁ h₂ h₃ =>
+    apply Deduction.comm 
+    apply Deduction.weak 
+    . sorry
+    . exact h₃ d₁ d₂
+  case comm A₁ Γ₁ n₁ n₂ A₂ A₃ t₃ h₁ h₂ => 
+    have : (n:A,n₁:A₂,n₂:A₃,Γ₁) ⊢ q ∶ B := h₂ d₁ d₂
+    have that : (n:A,n₁:A₂,n₂:A₃,Γ₁) ∼ (n:A,n₂:A₃,n₁:A₂,Γ₁) := th1        
+    exact eqCtxEqDeduction that this
+  case app => contradiction
+  case subst => contradiction
+  case abs t₂ n₁ Γ₁ B₁ B₂ h₁ h₂ h₃ h₄ =>
+    have thus₁ : t₂ = q := by injection d₁; assumption
+    have thus₂ : n₁  = n := by injection d₁; assumption
+    have that₁ : B₂ = B := by injection d₂; assumption
+    have that₂  : B₁ = A := by injection d₂; assumption
+    rw [← thus₁]
+    rw [← that₁]
+    rw [← thus₂]
+    rw [← that₂]
+    apply Deduction.weak 
+    . cases (ctxSoundness h₁)
+      case a.cons => assumption
+    . assumption
+    
+
+theorem invAbs : (Γ ⊢ λ(n).t ∶ A->B) → ((n:A, Γ) ⊢ t ∶ B) := by
+  sorry
 
 variable (B C : Typ)
 -- We verify some basic properties of β - reduction --
